wip [RsUpConv]; hopefully this set of invariants is a complete one..

src/RsUpConv.v
@@ -2,12 +2,64 @@ Require Import Peano_dec Omega List ListSupport.
 Require Import Common FMap.
 Require Import Syntax Semantics SemFacts StepM Invariant Serial SerialFacts.
 Require Import Reduction Commutativity QuasiSeq Topology.
-Require Import RqRsTopo RqRsFacts RqRsInvMsg RqRsInvAtomic.
+Require Import RqRsTopo RqRsFacts RqRsInvMsg RqRsInvLock RqRsInvAtomic.
 
 Set Implicit Arguments.
 
 Local Open Scope list.
 Local Open Scope fmap.
+
+Lemma upLockedNew_equiv_false:
+  forall (orqs1 orqs2: ORqs Msg) oidx,
+    (orqs1@[oidx] >>=[[]] (fun orq => orq))@[upRq] = 
+    (orqs2@[oidx] >>=[[]] (fun orq => orq))@[upRq] ->
+    UpLockedNew orqs1 orqs2 oidx ->
+    False.
+Proof.
+  unfold UpLockedNew; intros.
+  destruct (orqs2@[oidx]); simpl in *; auto.
+  destruct (orqs1@[oidx]); simpl in *; dest; auto.
+  congruence.
+Qed.
+
+Lemma upLockedNew_weakened_false:
+  forall (orqs1 orqs2: ORqs Msg) oidx,
+    orqs2@[oidx] >>=[[]] (fun orq => orq)@[upRq] = None ->
+    UpLockedNew orqs1 orqs2 oidx ->
+    False.
+Proof.
+  unfold UpLockedNew; intros.
+  destruct (orqs2@[oidx]); simpl in *; auto.
+  dest; auto.
+Qed.
+
+(** TODO: move to [Topology.v], the one in [RqRsInvSepO.v] as well. *)
+Lemma parent_parent_in_False:
+  forall dtr (Hwf: WfDTree dtr) oidx1 oidx2 oidx3,
+    parentIdxOf dtr oidx1 = Some oidx2 ->
+    parentIdxOf dtr oidx2 = Some oidx3 ->
+    In oidx3 (subtreeIndsOf dtr oidx1) ->
+    False.
+Proof.
+  intros.
+  pose proof (subtreeIndsOf_child_in Hwf _ H).
+  pose proof (subtreeIndsOf_child_SubList Hwf _ H0).
+  apply H3 in H2.
+  pose proof (subtreeIndsOf_In_each_other_eq Hwf _ _ H1 H2); subst.
+  eapply parentIdxOf_asym; eassumption.
+Qed.
+
+(** TODO: move to [RqRsInvAtomic.v] *)
+Lemma upLockedNew_in_history:
+  forall {oifc: OStateIfc} (sys: System oifc) st1 hst st2 oidx,
+    steps step_m sys st1 hst st2 ->
+    UpLockedNew (bst_orqs st1) (bst_orqs st2) oidx ->
+    In oidx (oindsOf hst).
+Proof.
+  intros.
+  destruct (in_dec idx_dec oidx (oindsOf hst)); auto.
+  exfalso; eapply steps_not_in_history_no_new_uplocks; eauto.
+Qed.
 
 Section RsUpConv.
   Context {oifc: OStateIfc}.
@@ -17,8 +69,49 @@ Section RsUpConv.
              (Hrrs: RqRsSys dtr sys).
 
   Section LockStatus.
-    Variables (orqs1 orqs2: ORqs Msg).
+    Variables (oinds: list IdxT) (orqs1 orqs2: ORqs Msg).
 
+    (** Intactness of the lock state *)
+
+    Definition UpLockIntact (oidx: IdxT) :=
+      (orqs1@[oidx] >>=[[]] (fun orq => orq))@[upRq] =
+      (orqs2@[oidx] >>=[[]] (fun orq => orq))@[upRq].
+    
+    Definition DownLockIntact (oidx: IdxT) :=
+      (orqs1@[oidx] >>=[[]] (fun orq => orq))@[downRq] =
+      (orqs2@[oidx] >>=[[]] (fun orq => orq))@[downRq].
+
+    Definition ULDLIntact :=
+      forall oidx,
+        UpLockedNew orqs1 orqs2 oidx ->
+        DownLockIntact oidx.
+
+    Definition ULNewOrNotCovered (oidx: IdxT) :=
+      UpLockedNew orqs1 orqs2 oidx \/ ~ In oidx oinds.
+
+    Definition RqUpULNew (eouts: list (Id Msg)) :=
+      forall oidx rqUp,
+        RqUpMsgFrom dtr oidx rqUp ->
+        In rqUp eouts ->
+        UpLockedNew orqs1 orqs2 oidx.
+
+    Definition RsDownULNew (eouts: list (Id Msg)) :=
+      forall oidx rsDown,
+        RsDownMsgTo dtr oidx rsDown ->
+        In rsDown eouts ->
+        ULNewOrNotCovered oidx.
+
+    Definition UpLockedNewChained :=
+      forall pidx orq rqiu,
+        UpLockedNew orqs1 orqs2 pidx ->
+        orqs2@[pidx] = Some orq -> orq@[upRq] = Some rqiu ->
+        forall cidx,
+          parentIdxOf dtr cidx = Some pidx ->
+          edgeDownTo dtr cidx = Some rqiu.(rqi_midx_rsb) ->
+          ULNewOrNotCovered cidx.
+
+    (** Newly downlocked states *)
+    
     Definition DownLockedNew (oidx: IdxT) :=
       orqs2@[oidx] >>=[False]
            (fun orq2 =>
@@ -41,6 +134,8 @@ Section RsUpConv.
           rsEdgeUpFrom dtr oidx = Some rqid.(rqi_midx_rsb) ->
           DownLockedNew pidx.
 
+    (** This invariant is the only necessary condition to prove non-mergeability,
+     * used in [RqRsCorrect.v] *)
     Definition RsUpDLNew (eouts: list (Id Msg)) :=
       forall oidx rsUp pidx,
         RsUpMsgFrom dtr oidx rsUp ->
@@ -48,9 +143,28 @@ Section RsUpConv.
         In rsUp eouts ->
         DownLockedNew pidx.
 
-    Definition DLNewOuts (eouts: list (Id Msg)) :=
-      RqDownDLNew eouts /\ DLDLNew /\ RsUpDLNew eouts.
+    Definition DLNewBackUpLockedNew :=
+      forall pidx orq rqid,
+        DownLockedNew pidx ->
+        orqs2@[pidx] = Some orq -> orq@[downRq] = Some rqid ->
+        forall cidx,
+          parentIdxOf dtr cidx = Some pidx ->
+          edgeDownTo dtr cidx = Some rqid.(rqi_midx_rsb) ->
+          ULNewOrNotCovered cidx.
 
+    (** All together *)
+
+    Definition DLOutsInv (eouts: list (Id Msg)) :=
+      RqUpULNew eouts /\
+      RsDownULNew eouts /\
+      RqDownDLNew eouts /\
+      RsUpDLNew eouts.
+
+    Definition DLLockInv :=
+      ULDLIntact /\ UpLockedNewChained /\
+      DLDLNew /\ DLNewBackUpLockedNew.
+
+    (* An orthogonal invariant, also required in proving non-mergeability *)
     Definition DLOldPreserved :=
       forall oidx rqid,
         DownLocked orqs1 oidx rqid ->
@@ -62,13 +176,79 @@ Section RsUpConv.
         ~ In idm inits.
 
     Definition DLTimeInv (inits eouts: list (Id Msg)) :=
-      DLTimeInits inits -> DLNewOuts eouts /\ DLOldPreserved.
+      DLTimeInits inits ->
+      DLOutsInv eouts /\ DLLockInv /\ DLOldPreserved.
     
   End LockStatus.
 
   (** Utility lemmas *)
 
-  Lemma downLockedNew_irrefl:
+  Lemma UpLockIntact_trans:
+    forall orqs1 orqs2 oidx,
+      UpLockIntact orqs1 orqs2 oidx ->
+      forall orqs3,
+        UpLockIntact orqs2 orqs3 oidx ->
+        UpLockIntact orqs1 orqs3 oidx.
+  Proof.
+    unfold UpLockIntact; intros; congruence.
+  Qed.
+
+  Lemma UpLockIntact_UpLockedNew_1:
+    forall orqs1 orqs2 oidx,
+      UpLockIntact orqs1 orqs2 oidx ->
+      forall orqs3,
+        UpLockedNew orqs2 orqs3 oidx ->
+        UpLockedNew orqs1 orqs3 oidx.
+  Proof.
+    unfold UpLockIntact, UpLockedNew; intros.
+    destruct (orqs3@[oidx]); simpl in *; dest; auto.
+    split; [assumption|].
+    destruct (orqs1@[oidx]), (orqs2@[oidx]); simpl in *; auto.
+    congruence.
+  Qed.
+
+  Lemma UpLockIntact_UpLockedNew_2:
+    forall orqs1 orqs2 oidx,
+      UpLockedNew orqs1 orqs2 oidx ->
+      forall orqs3,
+        UpLockIntact orqs2 orqs3 oidx ->
+        UpLockedNew orqs1 orqs3 oidx.
+  Proof.
+    unfold UpLockIntact, UpLockedNew; intros.
+    destruct (orqs2@[oidx]); simpl in *; dest; [|exfalso; auto].
+    destruct (orqs1@[oidx]), (orqs3@[oidx]); simpl in *; auto.
+    - split; auto; congruence.
+    - split; auto; congruence.
+  Qed.
+
+  Lemma step_not_in_history_up_lock_intact:
+    forall st1 oidx ridx rins routs st2 uidx,
+      step_m sys st1 (RlblInt oidx ridx rins routs) st2 ->
+      uidx <> oidx ->
+      UpLockIntact st1.(bst_orqs) st2.(bst_orqs) uidx.
+  Proof.
+    intros.
+    inv H; simpl in *.
+    red; intros; mred.
+  Qed.
+
+  Lemma steps_not_in_history_up_lock_intact:
+    forall st1 hst st2 oidx,
+      steps step_m sys st1 hst st2 ->
+      ~ In oidx (oindsOf hst) ->
+      UpLockIntact st1.(bst_orqs) st2.(bst_orqs) oidx.
+  Proof.
+    induction 1; simpl; intros; [red; reflexivity|].
+    destruct lbl; try (inv H0; simpl in *; auto; fail).
+    simpl in *.
+    eapply UpLockIntact_trans.
+    - eapply IHsteps; eauto.
+    - eapply step_not_in_history_up_lock_intact.
+      + apply H0.
+      + auto.
+  Qed.
+
+  Lemma DownLockedNew_not_refl:
     forall (orqs1 orqs2: ORqs Msg) oidx,
       (orqs1@[oidx] >>=[M.empty _] (fun orq => orq))@[downRq] =
       (orqs2@[oidx] >>=[M.empty _] (fun orq => orq))@[downRq] ->
@@ -82,7 +262,7 @@ Section RsUpConv.
     congruence.
   Qed.
 
-  Lemma downLockedNew_equiv:
+  Lemma DownLockedNew_equiv:
     forall (orqs1 porqs2: ORqs Msg) oidx,
       DownLockedNew orqs1 porqs2 oidx ->
       forall (norqs2: ORqs Msg),
@@ -98,7 +278,7 @@ Section RsUpConv.
     split; [congruence|auto].
   Qed.
 
-  Lemma downLocked_not_DownLockedNew:
+  Lemma DownLocked_not_DownLockedNew:
     forall orqs1 rqid orqs2 oidx,
       DownLocked orqs1 oidx rqid ->
       ~ DownLockedNew orqs1 orqs2 oidx.
@@ -110,7 +290,7 @@ Section RsUpConv.
     dest; congruence.
   Qed.
 
-  Lemma downLockedNew_DownLocked:
+  Lemma DownLockedNew_DownLocked:
     forall orqs1 orqs2 oidx,
       DownLockedNew orqs1 orqs2 oidx ->
       exists rqid, DownLocked orqs2 oidx rqid.
@@ -122,7 +302,96 @@ Section RsUpConv.
     exfalso; auto.
   Qed.
 
-  Lemma dlOldPreserved_orqs_eq:
+  Lemma DownLockIntact_trans:
+    forall orqs1 orqs2 oidx,
+      DownLockIntact orqs1 orqs2 oidx ->
+      forall orqs3,
+        DownLockIntact orqs2 orqs3 oidx ->
+        DownLockIntact orqs1 orqs3 oidx.
+  Proof.
+    unfold DownLockIntact; intros; congruence.
+  Qed.
+
+  Lemma DownLockIntact_DownLockedNew_1:
+    forall orqs1 orqs2 oidx,
+      DownLockIntact orqs1 orqs2 oidx ->
+      forall orqs3,
+        DownLockedNew orqs2 orqs3 oidx ->
+        DownLockedNew orqs1 orqs3 oidx.
+  Proof.
+    unfold DownLockIntact, DownLockedNew; intros.
+    destruct (orqs3@[oidx]); simpl in *; dest; auto.
+    split; [assumption|].
+    destruct (orqs1@[oidx]), (orqs2@[oidx]); simpl in *; auto.
+    congruence.
+  Qed.
+
+  Lemma DownLockIntact_DownLockedNew_2:
+    forall orqs1 orqs2 oidx,
+      DownLockedNew orqs1 orqs2 oidx ->
+      forall orqs3,
+        DownLockIntact orqs2 orqs3 oidx ->
+        DownLockedNew orqs1 orqs3 oidx.
+  Proof.
+    unfold DownLockIntact, DownLockedNew; intros.
+    destruct (orqs2@[oidx]); simpl in *; dest; [|exfalso; auto].
+    destruct (orqs1@[oidx]), (orqs3@[oidx]); simpl in *; auto.
+    - split; auto; congruence.
+    - split; auto; congruence.
+  Qed.
+
+  Lemma step_not_in_history_down_lock_intact:
+    forall st1 oidx ridx rins routs st2 uidx,
+      step_m sys st1 (RlblInt oidx ridx rins routs) st2 ->
+      uidx <> oidx ->
+      DownLockIntact st1.(bst_orqs) st2.(bst_orqs) uidx.
+  Proof.
+    intros.
+    inv H; simpl in *.
+    red; intros; mred.
+  Qed.
+
+  Lemma steps_not_in_history_down_lock_intact:
+    forall st1 hst st2 oidx,
+      steps step_m sys st1 hst st2 ->
+      ~ In oidx (oindsOf hst) ->
+      DownLockIntact st1.(bst_orqs) st2.(bst_orqs) oidx.
+  Proof.
+    induction 1; simpl; intros; [red; reflexivity|].
+    destruct lbl; try (inv H0; simpl in *; auto; fail).
+    simpl in *.
+    eapply DownLockIntact_trans.
+    - eapply IHsteps; eauto.
+    - eapply step_not_in_history_down_lock_intact.
+      + apply H0.
+      + auto.
+  Qed.
+
+  Lemma DownLockedNew_not_DownLockIntact:
+    forall orqs1 orqs2 oidx,
+      DownLockedNew orqs1 orqs2 oidx ->
+      ~ DownLockIntact orqs1 orqs2 oidx.
+  Proof.
+    unfold DownLockedNew, DownLockIntact; intros.
+    destruct (orqs2@[oidx]); simpl in *; dest; auto.
+    destruct (orqs1@[oidx]); simpl in *; auto.
+    congruence.
+  Qed.
+
+  Lemma DownLockedNew_in_history:
+    forall st1 hst st2 oidx,
+      steps step_m sys st1 hst st2 ->
+      DownLockedNew (bst_orqs st1) (bst_orqs st2) oidx ->
+      In oidx (oindsOf hst).
+  Proof.
+    intros.
+    destruct (in_dec idx_dec oidx (oindsOf hst)); auto.
+    exfalso.
+    eapply steps_not_in_history_down_lock_intact in H; [|eassumption].
+    eapply DownLockedNew_not_DownLockIntact; eauto.
+  Qed.
+
+  Lemma DLOldPreserved_orqs_equiv:
     forall (orqs1 orqs2: ORqs Msg),
       (forall oidx,
           (orqs1@[oidx] >>=[[]] (fun orq => orq))@[downRq] =
@@ -136,7 +405,7 @@ Section RsUpConv.
     destruct (orqs2@[oidx]); simpl in *; mred.
   Qed.
 
-  Lemma dlOldPreserved_new:
+  Lemma DLOldPreserved_new:
     forall (orqs: ORqs Msg) oidx orq rqid,
       (orqs@[oidx] >>=[[]] (fun orq => orq))@[downRq] = None ->
       orq@[downRq] = Some rqid ->
@@ -148,7 +417,7 @@ Section RsUpConv.
     simpl in *; exfalso; congruence.
   Qed.
 
-  Lemma dlOldPreserved_orqs_equiv:
+  Lemma DLOldPreserved_orqs_step:
     forall (orqs1 porqs2: ORqs Msg),
       DLOldPreserved orqs1 porqs2 ->
       forall (norqs2: ORqs Msg),
@@ -168,111 +437,104 @@ Section RsUpConv.
     destruct (norqs2@[oidx]); simpl in *; mred.
   Qed.
 
-  Lemma dlNewOuts_app:
-    forall orqs1 orqs2 eouts1 eouts2,
-      DLNewOuts orqs1 orqs2 eouts1 ->
-      DLNewOuts orqs1 orqs2 eouts2 ->
-      DLNewOuts orqs1 orqs2 (eouts1 ++ eouts2).
+  Lemma DLOutsInv_app:
+    forall oinds orqs1 orqs2 eouts1 eouts2,
+      DLOutsInv oinds orqs1 orqs2 eouts1 ->
+      DLOutsInv oinds orqs1 orqs2 eouts2 ->
+      DLOutsInv oinds orqs1 orqs2 (eouts1 ++ eouts2).
   Proof.
-    unfold DLNewOuts; intros; dest.
-    repeat ssplit; try assumption.
-    - red; intros.
-      apply in_app_or in H7; destruct H7; eauto.
-    - red; intros.
-      apply in_app_or in H7; destruct H7; eauto.
-  Qed.
-
-  Lemma dlNewOuts_removeOnce:
-    forall orqs1 orqs2 idm eouts,
-      DLNewOuts orqs1 orqs2 eouts ->
-      DLNewOuts orqs1 orqs2 (removeOnce (id_dec msg_dec) idm eouts).
-  Proof.
-    unfold DLNewOuts; intros; dest.
-    repeat ssplit; try assumption.
-    - red; intros.
-      apply removeOnce_In_2 in H4; eauto.
-    - red; intros.
-      apply removeOnce_In_2 in H4; eauto.
-  Qed.
-
-  Lemma dlNewOuts_removeL:
-    forall orqs1 orqs2 msgs eouts,
-      DLNewOuts orqs1 orqs2 eouts ->
-      DLNewOuts orqs1 orqs2 (removeL (id_dec msg_dec) eouts msgs).
-  Proof.
-    unfold DLNewOuts; intros; dest.
-    repeat ssplit; try assumption.
-    - red; intros.
-      apply removeL_In_2 in H4; eauto.
-    - red; intros.
-      apply removeL_In_2 in H4; eauto.
-  Qed.
-
-  Lemma dlDLNew_orqs_equiv:
-    forall (orqs1 porqs2: ORqs Msg),
-      DLDLNew orqs1 porqs2 ->
-      forall norqs2: ORqs Msg,
-        (forall oidx,
-            (porqs2@[oidx] >>=[[]] (fun orq => orq))@[downRq] =
-            (norqs2@[oidx] >>=[[]] (fun orq => orq))@[downRq]) ->
-        DLDLNew orqs1 norqs2.
-  Proof.
-    red; intros.
-    eapply downLockedNew_equiv; eauto.
-    specialize (H0 oidx).
-    rewrite H2 in H0; simpl in H0.
-    rewrite H3 in H0.
-    destruct (porqs2@[oidx]) as [porq2|] eqn:Hporq2; [|discriminate].
-    simpl in H0.
-    eapply H.
-    1: {
-      instantiate (1:= oidx).
-      eapply downLockedNew_equiv; eauto.
-      rewrite Hporq2, H2; simpl; congruence.
-    }
-    all: eassumption.
-  Qed.
-
-  Lemma dlNewOuts_orqs_equiv:
-    forall (orqs1 porqs2: ORqs Msg) eouts,
-      DLNewOuts orqs1 porqs2 eouts ->
-      forall norqs2: ORqs Msg,
-        (forall oidx,
-            (porqs2@[oidx] >>=[[]] (fun orq => orq))@[downRq] =
-            (norqs2@[oidx] >>=[[]] (fun orq => orq))@[downRq]) ->
-        DLNewOuts orqs1 norqs2 eouts.
-  Proof.
-    unfold DLNewOuts; intros; dest.
+    unfold DLOutsInv; intros; dest.
     repeat ssplit.
-    - red; intros.
-      eapply downLockedNew_equiv; eauto.
-    - eapply dlDLNew_orqs_equiv; eauto.
-    - red; intros.
-      eapply downLockedNew_equiv; eauto.
+    - red; intros; apply in_app_or in H8; destruct H8; eauto.
+    - red; intros; apply in_app_or in H8; destruct H8; eauto.
+    - red; intros; apply in_app_or in H9; destruct H9; eauto.
+    - red; intros; apply in_app_or in H9; destruct H9; eauto.
+  Qed.
+
+  Lemma DLOutsInv_removeOnce:
+    forall oinds orqs1 orqs2 eouts,
+      DLOutsInv oinds orqs1 orqs2 eouts ->
+      forall idm,
+        DLOutsInv oinds orqs1 orqs2 (removeOnce (id_dec msg_dec) idm eouts).
+  Proof.
+    unfold DLOutsInv; intros; dest.
+    repeat ssplit.
+    - red; intros; apply removeOnce_In_2 in H4; eauto.
+    - red; intros; apply removeOnce_In_2 in H4; eauto.
+    - red; intros; apply removeOnce_In_2 in H5; eauto.
+    - red; intros; apply removeOnce_In_2 in H5; eauto.
+  Qed.
+      
+  Lemma DLOutsInv_removeL:
+    forall oinds orqs1 orqs2 eouts,
+      DLOutsInv oinds orqs1 orqs2 eouts ->
+      forall msgs,
+        DLOutsInv oinds orqs1 orqs2 (removeL (id_dec msg_dec) eouts msgs).
+  Proof.
+    unfold DLOutsInv; intros; dest.
+    repeat ssplit; try assumption.
+    - red; intros; apply removeL_In_2 in H4; eauto.
+    - red; intros; apply removeL_In_2 in H4; eauto.
+    - red; intros; apply removeL_In_2 in H5; eauto.
+    - red; intros; apply removeL_In_2 in H5; eauto.
   Qed.
 
   Ltac disc_rule_custom ::=
     try disc_footprints_ok;
     try disc_msg_case.
-  
-  Ltac solve_RqDownDLNew_exfalso :=
-    match goal with
-    | |- RqDownDLNew _ _ _ =>
-      red; intros; dest_in; disc_rule_conds; solve_midx_false
-    end.
 
-  Ltac solve_RsUpDLNew_exfalso :=
-    match goal with
-    | |- RsUpDLNew _ _ _ =>
-      red; intros; dest_in; disc_rule_conds; solve_midx_false
-    end.
+  Ltac exfalso_wrong_msg_lock :=
+    red; intros; dest_in; disc_rule_conds; solve_midx_false;
+    try 
+      match goal with
+      | [H: UpLockedNew ?orqs ?orqs _ |- _] =>
+        exfalso; eapply upLockedNew_not_refl; eauto
+      | [H: DownLockedNew ?orqs ?orqs _ |- _] =>
+        exfalso; eapply DownLockedNew_not_refl; eauto
+      end.
+
+  Ltac smred := repeat (simpl in *; mred).
+
+  Hint Extern 1 (WfDTree dtr) => apply Hrrs.
+
+  Ltac disc_RqRsDownMatch_rq :=
+    repeat
+      match goal with
+      | [Hin: In _ ?outs, Hf: Forall _ ?outs |- _] =>
+        rewrite Forall_forall in Hf; specialize (Hf _ Hin)
+      end;
+    try
+      match goal with
+      | [Hin: In _ ?outs, Hrr: RqRsDownMatch _ _ (idsOf ?outs) _ _ |- _] =>
+        apply in_map with (f:= idOf) in Hin;
+        let Hrri := fresh "H" in
+        pose proof (RqRsDownMatch_rq_rs Hrr _ Hin) as Hrri;
+        let cidx := fresh "cidx" in
+        let rsUp := fresh "rsUp" in
+        destruct Hrri as [cidx [rsUp ?]]; dest
+      end.
+
+  Ltac exfalso_rqDown_rsUp :=
+    repeat
+      match goal with
+      | [H: Forall ?P _ |- _] =>
+        match P with
+        | context[RqDownMsgOutInv] => apply rqDown_rsUp_inv_msg in H
+        end
+      | [Hf: Forall (fun _ => exists _, RqDownRsUpIdx _ _ _) ?outs,
+             Hin: In _ ?outs |- _] =>
+        rewrite Forall_forall in Hf; specialize (Hf _ Hin);
+        let oidx := fresh "oidx" in destruct Hf as [oidx ?]
+      | [H1: RqDownRsUpIdx _ ?eouts ?idm, H2: RsDownMsgTo _ _ ?idm |- _] =>
+        destruct H1; disc_rule_conds; solve_midx_false
+      end.
 
   Lemma step_down_lock_time_ok:
     forall st1,
       Reachable (steps step_m) sys st1 ->
       forall oidx ridx rins routs st2,
         step_m sys st1 (RlblInt oidx ridx rins routs) st2 ->
-        DLTimeInv (bst_orqs st1) (bst_orqs st2) rins routs.
+        DLTimeInv [oidx] (bst_orqs st1) (bst_orqs st2) rins routs.
   Proof.
     destruct Hrrs as [? [? ?]].
     intros.
@@ -287,12 +549,11 @@ Section RsUpConv.
       disc_rule_conds.
       replace (orqs +[obj_idx obj <- norq]) with orqs by meq.
       red; intros _.
-      repeat split.
-      + solve_RqDownDLNew_exfalso.
-      + red; intros.
-        exfalso; eapply downLockedNew_irrefl; eauto.
-      + solve_RsUpDLNew_exfalso.
-      + apply dlOldPreserved_orqs_eq; auto.
+      repeat split; try (exfalso_wrong_msg_lock; fail).
+      + red; intros; dest_in; disc_rule_conds.
+        right; intro Hx; dest_in.
+        apply parentIdxOf_not_eq in H32; [|apply Hrrs].
+        auto.
 
     - (** case [ImmUp] *)
       disc_rule_conds.
@@ -304,40 +565,59 @@ Section RsUpConv.
       disc_rule_conds.
       + (** case [RqUpUp] *)
         red; intros _.
-        repeat split.
-        * solve_RqDownDLNew_exfalso.
-        * red; intros.
-          exfalso; eapply downLockedNew_irrefl; [|eassumption].
-          repeat (simpl; mred).
-          destruct (idx_dec oidx (obj_idx obj)); subst; mred.
-        * solve_RsUpDLNew_exfalso.
-        * apply dlOldPreserved_orqs_eq.
-          intros.
-          destruct (idx_dec oidx (obj_idx obj));
-            subst; repeat (simpl; mred).
+        repeat ssplit.
+        * red; repeat ssplit; try (exfalso_wrong_msg_lock; fail).
+          { red; intros; dest_in; disc_rule_conds.
+            red; smred; split; [discriminate|reflexivity].
+          }
+        * red; repeat ssplit.
+          { red; intros; red; smred. }
+          { red; intros.
+            red in H13; destruct (idx_dec pidx (obj_idx obj)); subst; smred.
+            right; intro Hx; dest_in.
+            apply parentIdxOf_not_eq in H25; auto.
+          }
+          { red; intros.
+            red in H13; destruct (idx_dec oidx (obj_idx obj)); subst; smred.
+          }
+          { red; intros.
+            red in H13; destruct (idx_dec pidx (obj_idx obj)); subst; smred.
+          }
+        * apply DLOldPreserved_orqs_equiv.
+          intros; smred.
 
       + (** case [RqUpDown] *)
         red; intros _.
-        repeat split.
-        * red; intros.
-          apply in_map with (f:= idOf) in H22.
-          eapply RqRsDownMatch_rq_rs in H19; [|eassumption].
-          destruct H19 as [cidx [rsUp ?]]; dest.
-          disc_rule_conds.
-          red; repeat (simpl; mred).
-          split; [discriminate|reflexivity].
-        * red; intros.
-          destruct (idx_dec oidx (obj_idx obj)).
-          { subst; mred; solve_midx_false. }
-          { exfalso; eapply downLockedNew_irrefl; [|eassumption].
-            repeat (simpl; mred).
+        repeat ssplit.
+        * red; repeat ssplit.
+          { red; intros; exfalso.
+            disc_RqRsDownMatch_rq; disc_rule_conds; solve_midx_false.
           }
-        * red; intros.
-          apply in_map with (f:= idOf) in H22.
-          eapply RqRsDownMatch_rq_rs in H19; [|eassumption].
-          destruct H19 as [cidx [rsUp' ?]]; dest.
-          disc_rule_conds; solve_midx_false.
-        * eapply dlOldPreserved_new; mred.
+          { red; intros; exfalso.
+            disc_RqRsDownMatch_rq; disc_rule_conds; solve_midx_false.
+          }
+          { red; intros.
+            disc_RqRsDownMatch_rq; disc_rule_conds.
+            red; smred; split; [discriminate|reflexivity].
+          }
+          { red; intros; disc_RqRsDownMatch_rq; disc_rule_conds. }
+        * red; repeat ssplit.
+          { red; intros; exfalso.
+            eapply upLockedNew_equiv_false; [|eassumption]; smred.
+          }
+          { red; intros; exfalso.
+            red in H4; destruct (idx_dec pidx (obj_idx obj)); subst; smred.
+          }
+          { red; intros; exfalso.
+            red in H4; destruct (idx_dec oidx (obj_idx obj)); subst; smred.
+            disc_rule_conds; solve_midx_false.
+          }
+          { red; intros.
+            red in H4; destruct (idx_dec pidx (obj_idx obj)); subst; smred.
+            right; intro Hx; dest_in.
+            apply parentIdxOf_not_eq in H25; auto.
+          }
+        * eapply DLOldPreserved_new; mred.
 
       + (** case [RqDownDown] *)
         red; intros; exfalso.
@@ -349,17 +629,31 @@ Section RsUpConv.
       disc_rule_conds.
       + (** case [RsDownDown] *)
         red; intros _.
-        repeat split.
-        * solve_RqDownDLNew_exfalso.
-        * red; intros.
-          exfalso; eapply downLockedNew_irrefl; [|eassumption].
-          repeat (simpl; mred).
-          destruct (idx_dec oidx (obj_idx obj)); subst; mred.
-        * solve_RsUpDLNew_exfalso.
-        * apply dlOldPreserved_orqs_eq.
-          intros.
-          destruct (idx_dec oidx (obj_idx obj));
-            subst; repeat (simpl; mred).
+        repeat ssplit.
+        * red; repeat ssplit; try (exfalso_wrong_msg_lock; fail).
+          { red; intros; dest_in; disc_rule_conds.
+            right; intro Hx; dest_in.
+            apply parentIdxOf_not_eq in H4; auto.
+          }
+        * red; repeat ssplit.
+          { red; intros; exfalso.
+            destruct (idx_dec oidx (obj_idx obj)); subst.
+            { eapply upLockedNew_weakened_false; [|eassumption]; smred. }
+            { eapply upLockedNew_equiv_false; [|eassumption]; smred. }
+          }
+          { red; intros; exfalso.
+            destruct (idx_dec pidx (obj_idx obj)); subst.
+            { eapply upLockedNew_weakened_false; [|eassumption]; smred. }
+            { eapply upLockedNew_equiv_false; [|eassumption]; smred. }
+          }
+          { red; intros; exfalso.
+            red in H23; destruct (idx_dec oidx (obj_idx obj)); subst; smred.
+          }
+          { red; intros; exfalso.
+            red in H23; destruct (idx_dec pidx (obj_idx obj)); subst; smred.
+          }
+        * eapply DLOldPreserved_orqs_equiv.
+          intros; smred.
 
       + (** case [RsUpDown] *)
         red; intros; exfalso.
@@ -386,29 +680,32 @@ Section RsUpConv.
     - (** case [RsDownRqDown] *)
       disc_rule_conds.
       red; intros _.
-      repeat split.
-      * red; intros.
-        apply in_map with (f:= idOf) in H22.
-        eapply RqRsDownMatch_rq_rs in H19; [|eassumption].
-        destruct H19 as [cidx [rsUp ?]]; dest.
-        disc_rule_conds.
-        red; repeat (simpl; mred).
-        split; [discriminate|reflexivity].
-      * red; intros.
-        destruct (idx_dec oidx (obj_idx obj)).
-        { subst; mred.
-          rewrite H36 in *.
-          solve_midx_false.
-        }
-        { exfalso; eapply downLockedNew_irrefl; [|eassumption].
-          repeat (simpl; mred).
-        }
-      * red; intros.
-        apply in_map with (f:= idOf) in H22.
-        eapply RqRsDownMatch_rq_rs in H19; [|eassumption].
-        destruct H19 as [cidx [rsUp' ?]]; dest.
-        disc_rule_conds; solve_midx_false.
-      * eapply dlOldPreserved_new; mred.
+      repeat ssplit.
+      + red; repeat ssplit.
+        * red; intros; exfalso.
+          disc_RqRsDownMatch_rq; disc_rule_conds; solve_midx_false.
+        * red; intros; exfalso.
+          disc_RqRsDownMatch_rq; disc_rule_conds; solve_midx_false.
+        * red; intros.
+          disc_RqRsDownMatch_rq; disc_rule_conds.
+          red; smred; split; [discriminate|reflexivity].
+        * red; intros; disc_RqRsDownMatch_rq; disc_rule_conds.
+      + red; repeat ssplit.
+        * red; intros; exfalso.
+          destruct (idx_dec oidx (obj_idx obj)); subst.
+          { eapply upLockedNew_weakened_false; [|eassumption]; smred. }
+          { eapply upLockedNew_equiv_false; [|eassumption]; smred. }
+        * red; intros; exfalso.
+          red in H4; destruct (idx_dec pidx (obj_idx obj)); subst; smred.
+        * red; intros; exfalso.
+          red in H4; destruct (idx_dec oidx (obj_idx obj)); subst; smred.
+          disc_rule_conds; solve_midx_false.
+        * red; intros.
+          red in H4; destruct (idx_dec pidx (obj_idx obj)); subst; smred.
+          right; intro Hx; dest_in.
+          apply parentIdxOf_not_eq in H23; auto.
+      + eapply DLOldPreserved_new; mred.
+
   Qed.
 
   Lemma atomic_down_lock_time_ok:
@@ -417,7 +714,7 @@ Section RsUpConv.
       forall st1 st2,
         Reachable (steps step_m) sys st1 ->
         steps step_m sys st1 hst st2 ->
-        DLTimeInv st1.(bst_orqs) st2.(bst_orqs) inits eouts.
+        DLTimeInv (oindsOf hst) st1.(bst_orqs) st2.(bst_orqs) inits eouts.
   Proof.
     destruct Hrrs as [? [? ?]].
     induction 1; simpl; intros; subst;
@@ -425,7 +722,10 @@ Section RsUpConv.
     inv_steps.
     specialize (IHAtomic _ _ H8 H10).
 
-    pose proof (footprints_ok Hiorqs H0 H8) as Hftinv.
+    pose proof (footprints_ok Hiorqs H0 H8) as Hftinv0.
+    pose proof (footprints_ok Hiorqs H0 (reachable_steps H8 H10)) as Hftinv1.
+    pose proof (downLockInv_ok Hiorqs H0 H (proj2 H1)
+                               (reachable_steps H8 H10)) as Hdlinv.
     pose proof (atomic_msg_outs_ok Hiorqs Hrrs H2 H8 H10) as Hmoinv.
     
     inv_step.
@@ -434,61 +734,135 @@ Section RsUpConv.
 
     - (** case [ImmDown] *)
       disc_rule_conds.
-      replace (orqs +[obj_idx obj <- norq]) with orqs by meq.
-      red; intros.
-      specialize (IHAtomic H5); dest.
-      split.
-      + apply dlNewOuts_app.
-        * apply dlNewOuts_removeOnce; auto.
-        * repeat split.
-          { solve_RqDownDLNew_exfalso. }
-          { apply H6. }
-          { solve_RsUpDLNew_exfalso. }
-      + assumption.
+      inv Hmoinv; [|disc_rule_conds|].
+      2: {
+        simpl in *.
+        apply rqDown_rsUp_inv_msg in H6; rewrite Forall_forall in H6.
+        apply SubList_singleton_In in H4.
+        specialize (H6 _ H4); destruct H6 as [oidx ?].
+        destruct H6; disc_rule_conds; solve_midx_false.
+      }
+      apply SubList_singleton in H4; subst.
+      rewrite removeOnce_nil; simpl.
 
-    - (** case [ImmUp] *)
       disc_rule_conds.
       replace (orqs +[obj_idx obj <- norq]) with orqs by meq.
       red; intros.
       specialize (IHAtomic H5); dest.
-      split.
-      + apply dlNewOuts_app.
-        * apply dlNewOuts_removeOnce; auto.
-        * red; repeat ssplit.
-          { solve_RqDownDLNew_exfalso. }
-          { apply H6. }
-          { red; intros; dest_in; disc_rule_conds.
-            red in H6; dest.
-            eapply H6 with (rqDown:= (rqFrom, rqm)).
-            { red; eauto. }
-            { assumption. }
-            { apply SubList_singleton_In; assumption. }
-          }
+      red in H26, H27; dest.
+      repeat ssplit.
+      + red; repeat ssplit; try (exfalso_wrong_msg_lock; fail).
+        red; intros; dest_in; disc_rule_conds.
+        left; eapply H26; [|left; reflexivity].
+        red; auto.
+      + red; repeat ssplit; try assumption.
+        * red; intros.
+          specialize (H30 _ _ _ H38 H39 H40 _ H41 H42).
+          destruct H30; [left; assumption|].
+          right; intro Hx; icase cidx; auto.
+          eapply upLockedNew_in_history in H10; [|eassumption].
+          apply H14 in H10.
+          eapply parent_parent_in_False
+            with (dtr:= dtr) (oidx2:= obj_idx obj); eauto.
+        * red; intros.
+          specialize (H32 _ _ _ H38 H39 H40 _ H41 H42).
+          destruct H32; [left; assumption|].
+          right; intro Hx; icase cidx; auto.
+          eapply DownLockedNew_in_history in H10; [|eassumption].
+          eapply parent_parent_in_False
+            with (dtr:= dtr) (oidx2:= obj_idx obj); eauto.
+      + assumption.
+
+    - (** case [ImmUp] *)
+      disc_rule_conds.
+      inv Hmoinv; [disc_rule_conds; solve_midx_false|disc_rule_conds|].
+      apply SubList_singleton_In in H4.
+
+      replace (orqs +[obj_idx obj <- norq]) with orqs by meq.
+      red; intros.
+      specialize (IHAtomic H21); dest.
+      red in H25, H27; dest.
+      repeat ssplit.
+
+      + apply DLOutsInv_app; [apply DLOutsInv_removeOnce|].
+        * red; repeat ssplit; try assumption.
+          red; intros; exfalso_rqDown_rsUp.
+        * red; repeat ssplit; try (exfalso_wrong_msg_lock; fail).
+          red; intros; dest_in; disc_rule_conds.
+          eapply H34; eauto.
+          red; auto.
+
+      + red; repeat ssplit; try assumption.
+        * red; intros.
+          specialize (H29 _ _ _ H36 H37 H38 _ H39 H40).
+          destruct H29; [left; assumption|].
+          right; intro Hx; icase cidx; auto.
+          apply H27 in H36.
+          eapply DownLockedNew_not_DownLockIntact; [|eassumption].
+          eapply H34; [|eassumption|eassumption].
+          red; auto.
+        * red; intros.
+          specialize (H31 _ _ _ H36 H37 H38 _ H39 H40).
+          destruct H31; [left; assumption|].
+          right; intro Hx; icase cidx; auto.
+          (* clear Hftinv0; good_footprint_get pidx. *)
+          (* disc_rule_conds. *)
+          admit. (** Need to know [~ In (rqi_midx_rsb rqid) (rqi_minds_rss rqid)] *)
+
       + assumption.
 
     - (** case [RqFwd] *)
       disc_rule_conds.
       + (** case [RqUpUp] *)
+        inv Hmoinv; [|disc_rule_conds|].
+        2: {
+          simpl in *.
+          apply rqDown_rsUp_inv_msg in H23; rewrite Forall_forall in H23.
+          apply SubList_singleton_In in H4.
+          specialize (H23 _ H4); destruct H23 as [oidx ?].
+          destruct H23; disc_rule_conds; solve_midx_false.
+        }
+        apply SubList_singleton in H4; subst.
+        rewrite removeOnce_nil; simpl.
+
+        disc_rule_conds.
         red; intros.
         specialize (IHAtomic H17); dest.
-        split.
-        * apply dlNewOuts_app.
-          { apply dlNewOuts_removeOnce.
-            eapply dlNewOuts_orqs_equiv; eauto.
-            intros; repeat (simpl; mred).
+        red in H33, H34; dest.
+        repeat ssplit.
+        * red; repeat ssplit; try (exfalso_wrong_msg_lock; fail).
+          red; intros; dest_in; disc_rule_conds.
+          eapply UpLockIntact_UpLockedNew_1.
+          { eapply steps_not_in_history_up_lock_intact; [eassumption|].
+            intro Hx; apply H29 in Hx.
+            eapply parent_not_in_subtree with (dtr:= dtr); eauto.
           }
-          { repeat split.
-            { solve_RqDownDLNew_exfalso. }
-            { eapply dlDLNew_orqs_equiv; [apply H23|].
-              intros; repeat (simpl; mred).
+          { simpl; red; intros; smred; split; [discriminate|reflexivity]. }
+        * red; repeat ssplit.
+          { red; intros.
+            destruct (idx_dec oidx0 (obj_idx obj)); subst.
+            { eapply DownLockIntact_trans.
+              { eapply steps_not_in_history_down_lock_intact; [eassumption|].
+                intro Hx; apply H29 in Hx.
+                eapply parent_not_in_subtree with (dtr:= dtr); eauto.
+              }
+              { simpl; red; intros; smred. }
             }
-            { solve_RsUpDLNew_exfalso. }
+            { eapply UpLockIntact_UpLockedNew_2
+                with (orqs3:= orqs) in H43; [|red; smred].
+              eapply DownLockIntact_trans with (orqs2:= orqs);
+                [apply H34; assumption|].
+              red; smred.
+            }
           }
-        * eapply dlOldPreserved_orqs_equiv; [eassumption|].
-          intros; repeat (simpl; mred).
+          { admit. }
+          { admit. }
+          { admit. }
+
+        * eapply DLOldPreserved_orqs_step; [eassumption|].
+          intros; smred.
 
       + (** case [RqUpDown] *)
-        (* .. Ltac? *)
         inv Hmoinv; [|disc_rule_conds|].
         2: {
           apply rqDown_rsUp_inv_msg in H17; rewrite Forall_forall in H17.
@@ -502,26 +876,9 @@ Section RsUpConv.
 
         red; intros.
         specialize (IHAtomic H6); dest.
-        red in H32; dest.
-
-        split.
-        * repeat split.
-          { (** TODO: need to substitute [bst_orqs st1] to [orqs]
-             * by proving a lemma that relates [DLNewOuts] and [steps] *)
-            admit.
-          }
-          { red; intros.
-            destruct (idx_dec oidx (obj_idx obj)).
-            { subst; mred; solve_midx_false. }
-            { admit. }
-          }
-          { red; intros; exfalso.
-            apply in_map with (f:= idOf) in H39.
-            eapply RqRsDownMatch_rq_rs in H23; [|eassumption].
-            destruct H23 as [cidx [rsUp' ?]]; dest.
-            disc_rule_conds; solve_midx_false.
-          }
-        * admit.
+        red in H32, H33; dest.
+        repeat ssplit.
+        all: admit.
 
       + (** case [RqDownDown] *)
         admit.
@@ -580,7 +937,7 @@ Section Corollaries.
     eapply atomic_down_lock_time_ok in H7; eauto.
     specialize (H7 H5); dest.
     red in H1; dest.
-    eapply H9; eauto.
+    eapply H11; eauto.
   Qed.
 
   Corollary extAtomic_rsUp_down_lock_preserved:
@@ -599,7 +956,7 @@ Section Corollaries.
     inv H1.
     eapply atomic_down_lock_time_ok in H5; eauto.
     specialize (H5 H3); dest.
-    apply H5; assumption.
+    apply H6; assumption.
   Qed.
 
   Lemma extAtomic_multi_rsUps_not_diverged_sub:
@@ -624,7 +981,7 @@ Section Corollaries.
     eapply steps_split in H1; [|reflexivity].
     destruct H1 as [sti1 [? ?]].
     eapply extAtomic_down_lock_time_ok with (rsUp:= rsUp1) in H0; eauto.
-    apply downLockedNew_DownLocked in H0.
+    apply DownLockedNew_DownLocked in H0.
     destruct H0 as [rqid ?].
 
     eapply steps_split in H11; [|reflexivity].
@@ -647,7 +1004,7 @@ Section Corollaries.
     eapply extAtomic_down_lock_time_ok
       with (rsUp:= rsUp2) (st1:= sti2) (st2:= st2) in H2; eauto;
       [|eapply reachable_steps; [|eassumption]; eauto].
-    eapply downLocked_not_DownLockedNew; eauto.
+    eapply DownLocked_not_DownLockedNew; eauto.
   Qed.
 
   Lemma extAtomic_multi_rsUps_not_diverged_gt:
